tests/lean/lakefile.lean
@@ -19,6 +19,7 @@ package «tests» {}
 @[default_target] lean_lib Bst
 @[default_target] lean_lib Builtin
 @[default_target] lean_lib BuiltinAuto
+@[default_target] lean_lib CastSigned
 @[default_target] lean_lib ChunksExact
 @[default_target] lean_lib Issue804ClosureReturnRef
 @[default_target] lean_lib Closures
